snapshot

JS.Ast.fst
@@ -2,26 +2,69 @@ module JS.Ast
 
 open FStar.String
 open FStar.List.Tot
+module R = FStar.Reflection
+open Output
 
-type mrange = int * int * int
-
-type js_unary_op = | JsUnary_Minus | JsUnary_Plus | JsUnary_Not | JsUnary_TypeOf
+type js_unary_op = 
+  | JsUnary_Minus | JsUnary_Plus | JsUnary_Not | JsUnary_TypeOf
+  | JsUnary_New
 type js_binary_op =
-  | JsBin_Eq | JsBin_Lt | JsBin_Le | JsBin_Gt | JsBin_Ge | JsBin_And | JsBin_Or
-  | JsBin_Minus | JsBin_Plus | JsBin_Mul | JsBin_Div | JsBin_InstanceOf
+  | JsBin_LooseEq | JsBin_Eq
+  | JsBin_Lt | JsBin_Le | JsBin_Gt | JsBin_Ge | JsBin_And | JsBin_Or
+  | JsBin_Minus | JsBin_Plus | JsBin_Mul | JsBin_Div
+  | JsBin_Rem | JsBin_Exp
+  | JsBin_InstanceOf
+  | JsBin_FunctionCall
+  | JsBin_MemberAccess
+  | JsBin_ComputedMemberAccess
+  | JsBin_Assign
+  | JsBin_Sequence
 
-type js_id = | JSId : range:option mrange -> s:string -> js_id
+type associatvity = | LeftToRight | RightToLeft
+
+let precedence_of_unary_op = function
+  | JsUnary_Not    -> 17, Some RightToLeft
+  | JsUnary_Plus   -> 17, Some RightToLeft
+  | JsUnary_Minus  -> 17, Some RightToLeft
+  | JsUnary_TypeOf -> 17, Some RightToLeft
+  | JsUnary_New    -> 19, Some RightToLeft
+
+let precedence_of_binary_op = function
+  | JsBin_Sequence             -> 1, Some LeftToRight
+  | JsBin_Assign               -> 3, Some RightToLeft
+  | JsBin_And                  -> 7, Some LeftToRight
+  | JsBin_Or                   -> 8, Some LeftToRight
+  | JsBin_LooseEq              -> 11, Some LeftToRight
+  | JsBin_Eq                   -> 11, Some LeftToRight
+  | JsBin_Lt                   -> 12, Some LeftToRight
+  | JsBin_Le                   -> 12, Some LeftToRight
+  | JsBin_Gt                   -> 12, Some LeftToRight
+  | JsBin_Ge                   -> 12, Some LeftToRight
+  | JsBin_InstanceOf           -> 12, Some LeftToRight
+  | JsBin_Minus                -> 14, Some LeftToRight
+  | JsBin_Plus                 -> 14, Some LeftToRight
+  | JsBin_Mul                  -> 15, Some LeftToRight
+  | JsBin_Exp                  -> 15, Some RightToLeft
+  | JsBin_Div                  -> 15, Some LeftToRight
+  | JsBin_Rem                  -> 15, Some LeftToRight
+  | JsBin_FunctionCall         -> 20, Some LeftToRight
+  | JsBin_MemberAccess         -> 20, Some LeftToRight
+  | JsBin_ComputedMemberAccess -> 20, Some LeftToRight
+
+type js_id = | JSId : range:option range_info -> s:string -> js_id
              | ReservedId : nat -> js_id
 
+let js_id_eq (i j: js_id)
+  = match i, j with
+  | JSId ir is, JSId jr js -> is = js
+  | ReservedId i, ReservedId j -> i = j
+  | _ -> false
+
 type js_expr
-  = | EAbs: args: list js_id -> body: js_expr -> js_expr
+  = | EArrowFun: args: list js_id -> body: js_expr -> js_expr
     | EFunction: fn:js_function -> js_expr
     | EVar: name: js_id -> js_expr
-    | EApp: f:js_expr -> this:js_expr -> args:list js_expr -> js_expr
-    | ENew: cons:js_expr -> args:list js_expr -> js_expr
-    | EGet: o:js_expr -> key:js_expr -> js_expr
-    | EAssign: o:js_expr -> v:js_expr -> js_expr
-    | ESeq: a:js_expr -> b:js_expr -> js_expr
+    | EApp: fn: js_expr -> args: list js_expr -> js_expr
     | EUnaryOp: op:js_unary_op -> v:js_expr -> js_expr
     | EBinaryOp: op:js_binary_op -> v:js_expr -> w:js_expr -> js_expr
     | EConst: c: js_const -> js_expr
@@ -43,5 +86,4 @@ and js_const =
     | CString: string -> js_const
     | CInt: int -> js_const
     | CBool: bool -> js_const
-
 
