JS.Translate.fst
@@ -1,331 +1,28 @@
 module JS.Translate
 
+open FStar.Tactics
 open FStar.List.Tot
 open JS.Ast
 open JS.Ast.Utils
 module O = Output
-
-type constructor
-  = { name: js_id
-    ; args: list (bool & js_id)
-    }
-type constructor_dico = list constructor
-    
-let mkCons (c: constructor) (args: list js_expr): js_expr
-  = ENew (EVar c.name) args
-
-let instanceOfCons (v: js_expr) (c: constructor): js_expr
-  = EBinaryOp JsBin_InstanceOf v (EGet (EVar c.name) (str "t"))
-
-let enable_optional_implicit = false
-
-let make_implicit_abs v (body: js_expr) (count: nat): nat & js_expr =
-  if enable_optional_implicit
-  then begin
-  let count = count + 1 in
-  // let  = ReservedId count in
-  // let count = count + 1 in
-  let bodyHolder = ReservedId count in
-  count,
-  EApp (eFunction None [] (
-    sseq
-      [ SLet v null
-      ; SLet bodyHolder body
-      ; SAssign (EGet (EVar bodyHolder) (str "feedImplicit")) (eFunction None [v] (
-                // TODO: here body is duplicated, we could circumvent
-                // this by having a binding `bodyHolder = v => body v`
-                // However, we should NOT set a new value to `v`
-                SReturn body
-        ))
-      ; SReturn (EVar bodyHolder)
-      ]
-  )) null []
-  end else count, (eFunction None [v] (SReturn body))
-
-let make_implicit_app f implicit_arg: js_expr
-  = if enable_optional_implicit
-    then
-    let feedImplicit = EGet f (str "feedImplicit") in
-    EApp (EBinaryOp JsBin_Or feedImplicit f) null [implicit_arg]
-    else EApp f null [implicit_arg]
-
-let js_of_constructor (c: constructor)
-  = let thisCons = sFunction (Some c.name) (map snd c.args) (
-        let assign_arg (arg: js_id) = ( (EConst CThis `EGet` idname arg) `SAssign` EVar arg) in
-         sseq (map assign_arg (map snd c.args))
-      ) in
-    let mk_e body (explicit, arg) = 
-      if explicit then eFunction None [arg] (SReturn body)
-      else snd (make_implicit_abs arg body 0)
-    in
-    let mk_curried args body = fold_left mk_e body (rev args) in
-    let creatorLet = JSId None "creator" in
-    let creator = mk_curried c.args (
-      ENew (EVar c.name) (map EVar (map snd c.args))
-    ) in
-    SLet c.name (wrap_as_expr (
-       sseq
-         [ thisCons
-         ; SLet creatorLet creator
-         ; SAssign (EGet (EVar creatorLet) (str "t")) (EVar c.name)
-         ; SReturn (EVar creatorLet)
-         ]
-    ))
-
-type pattern_match =
-    | JPat_Constant : js_expr -> pattern_match
-    | JPat_Cons     : constructor -> list pattern_match -> pattern_match
-    | JPat_Var      : js_id -> pattern_match
-
-let rec zip (a: list 'a) (b: list 'b) =
-  match a, b with
-  | a_hd::a_tl, b_hd::b_tl -> (a_hd,b_hd)::zip a_tl b_tl
-  | _ -> []
-  
-let rec js_condition_of_pattern_match (p: pattern_match) (head: js_expr): Tot js_expr (decreases p)
-  = match p with
-  | JPat_Constant e -> head ===. e
-  | JPat_Cons cons args -> fold_left (fun acc (pat, name) -> acc &&. js_condition_of_pattern_match (admit (); pat) (EGet head (idname name)))
-                                    (head `instanceOfCons` cons)
-                                    (zip args (map snd cons.args))
-  | JPat_Var _ -> EConst (CBool true)
-
-let rec js_bindings_of_pattern_match (p: pattern_match) (head: js_expr)
-  : Tot (list (js_id * js_expr)) (decreases p)
-  = match p with
-  | JPat_Constant e -> []
-  | JPat_Cons cons args -> fold_left (fun acc (pat, name) -> acc @ js_bindings_of_pattern_match (admit (); pat) (EGet head (idname name)))
-                                    []
-                                    (zip args (map snd cons.args))
-  | JPat_Var v -> [(v, head)]
-
-let js_of_pattern_match (p: pattern_match) (head: js_expr) (body: js_expr)
-  = let cond = js_condition_of_pattern_match p head in
-    let bindings = js_bindings_of_pattern_match p head in
-    let letClauses = fold_left (fun p (v, e) -> if p = SNoOp then SLet v e else p `SSeq` SLet v e) SNoOp bindings in
-    let body = letClauses `SSeq` SReturn body in
-    SIf cond body None
-
-
-let js_of_patterns_match (pb: list (pattern_match * js_expr)) (head: js_expr) (counter: nat)
-  : nat * js_expr
-  = let counter = counter + 1 in
-    counter,
-    wrap_as_expr begin
-      let let_temp = SLet (ReservedId counter) head in
-      let head = EVar (ReservedId counter) in
-      let branches = map (fun (pat, body) -> js_of_pattern_match pat head body) pb in
-      let_temp      `SSeq`
-      sseq branches `SSeq`
-      SThrow (
-        EBinaryOp JsBin_Plus
-          (str "Failed to pattern match ")
-          (head `EGet` str "constructor" `EGet` str "name")
-      )
-    end
-
-
-
-
-
-
-
-
-
-
-
-
-
-
-
-
-let c_unit =
-  { name = JSId None "Unit"
-  ; args = []
-  }
-
-open FStar.Tactics
-open FStar.List.Tot
-let vconst_to_js_ast (c: vconst) =
-  match c with
-  | C_Unit      -> mkCons c_unit []
-  | C_Int     i -> EConst (CInt i)
-  | C_True      -> EConst (CBool true)
-  | C_False     -> EConst (CBool false)
-  | C_String  s -> EConst (CString s)
-  | C_Range   r -> EConst (CString "!RANGE!")
-  | C_Reify     -> EConst (CString "!REIFY!")
-  | C_Reflect _ -> EConst (CString "!REFLECT!")
-
-
-
-let rec branch_to_js_pattern_match (dico: constructor_dico) (pat: pattern)
-  : Tac _
-  =
-  match pat with
-  | Pat_Constant vc -> JPat_Constant (vconst_to_js_ast vc)
-  | Pat_Cons fv args -> 
-         let name = fv_to_js_id fv in
-         ( match find (fun c -> c.name=name) dico with
-         | Some c -> 
-             JPat_Cons c
-                       (Tactics.map (fun (a, _) -> branch_to_js_pattern_match dico a)
-                       (admit (); args))
-         | _ -> fail ("The constructor " ^ name_of_jsid name ^ " was not found in the supplied constructor dictionnary!" )
-         )
-  | Pat_Var bv | Pat_Wild bv | Pat_Dot_Term bv _ -> JPat_Var (bv_to_js_id bv)
-
-let rec term_to_js_ast' (dico: constructor_dico) (t: term) (count: nat)
-  : Tac (nat & js_expr)
-  = let recurse t count = term_to_js_ast' dico t count in
-    match inspect t with
-  | Tv_Var   v | Tv_BVar  v -> count, EVar (bv_to_js_id v)
-  | Tv_FVar  v -> count, EVar (fv_to_js_id v)
-  | Tv_App   hd (arg, aqual) -> 
-    let count, hd = recurse hd count in
-    let count, arg = recurse arg count in
-    count, 
-    ( match aqual with
-    | Q_Explicit -> EApp hd null [arg]
-    | _ -> make_implicit_app hd arg)
-  | Tv_Abs   bv body -> 
-    let count, body = recurse body count in
-    let jid = binder_to_js_id bv in
-    ( match inspect_binder bv with
-    | _, Q_Explicit -> count, EAbs [jid] body
-    | _ -> make_implicit_abs jid body count
-    )
-  | Tv_Arrow _ _ | Tv_Type _ | Tv_Refine _ _ | Tv_AscribedT _ _ _ | Tv_AscribedC _ _ _ | Tv_Uvar  _ _ -> count, null
-  | Tv_Const c -> count, vconst_to_js_ast c
-  | Tv_Let r _ bv def body -> 
-    let count, body = recurse body count in
-    let count, def = recurse def count in
-    (if r then elet' else elet_nonrec) (bv_to_js_id bv) def body count
-  | Tv_Unknown -> count, wrap_as_expr (SThrow (str "cannot translate Tv_Unknown"))
-  | Tv_Match scrutinee brs -> 
-             let count, branches = Tactics.fold_left (fun (count, l) (pat, body) -> 
-                 let count, t = recurse body count in
-                 count, l@[branch_to_js_pattern_match dico pat, t]
-               ) (0,[]) brs in
-             let count, scrutinee = recurse scrutinee count in
-             js_of_patterns_match branches scrutinee count
-
-let term_to_js_ast (dico: constructor_dico) (t: term)
-  : Tac js_expr
-  = snd (term_to_js_ast' dico t 0)
-
-
-
-
-
-
-
-
-
-
-
-
-
-
-
-
-
-
-
-
-
-
-
-
-
-
-
-let constructor_names_of_sigelt (se: sigelt): Tac (list (name & typ))
-  = match inspect_sigelt se with
-  | Sg_Inductive _ _ _ _ cts -> cts
-  | _ -> fail "sigelt not an inductive" 
-
-
-let constructor_names_of_type_name (n: name): Tac (list (name & typ))
-  = match lookup_typ (top_env ()) n with
-  | Some n -> constructor_names_of_sigelt n
-  | _ -> fail "name not found"
-
-let mk_js_constructor (n: name) (t: typ)
-  : Tac constructor
+open JS.Translate.Constructor
+open JS.Translate.Term
+open JS.Translate.Helpers
+
+let mk_js_constructor (n: name) (t: typ): Tac constructor
   = let bds, _ = collect_arr_bs t in
     { name = fv_to_js_id (pack_fv n)
-    ; args = map (fun b -> 
+    ; args = Tactics.map (fun b -> 
            let _, q = inspect_binder b in
            ( match q with
            | Q_Explicit -> true
            | _ -> false
-           ), JSId None (name_of_binder b)
+           ), JSId (Some (O.range_to_range_info (range_of_binder b))) (name_of_binder b)
       ) bds
     }
 
-let mk_js_constructors (l: list (name & typ))
-  : Tac (list constructor)
-  = Tactics.map (fun (n, t) -> mk_js_constructor n t) l 
-
-let constructors_of_type_names (n: list name): Tac (list constructor)
-  = flatten (Tactics.map mk_js_constructors (Tactics.map constructor_names_of_type_name n))
-
 let js_of_sg_view_let  (dico: constructor_dico) (se: sigelt_view {Sg_Let? se}): Tac (js_stmt)
   = let Sg_Let r fv _ _ def = se in SLet (fv_to_js_id fv) (term_to_js_ast dico def)
-
-
-let rec (@@) (#a: eqtype) (l1 l2: list a): Tot (list a) (decreases l2) = 
-  match l2 with | [] -> l1
-                | hd::tl -> if mem hd l1 then l1 @@ tl
-                          else (hd::l1) @@ tl
-
-
-let rec collect_names (t: term)
-  : Tac (list name)
-  = match inspect t with
-  | Tv_FVar  v -> [inspect_fv v]
-  | Tv_App   hd (arg, _) -> collect_names hd @@ collect_names arg
-  | Tv_Abs   _ body -> collect_names body
-  | Tv_Let _ _ _ def body -> collect_names def @@ collect_names body
-  | Tv_Arrow _ _ | Tv_Type _ | Tv_Refine _ _ | Tv_AscribedT _ _ _ | Tv_AscribedC _ _ _ | Tv_Uvar _ _ | Tv_Var _ | Tv_BVar _ | Tv_Const _ | Tv_Unknown -> []
-  | Tv_Match scrutinee brs -> Tactics.fold_left (fun l b -> l @@ collect_names_of_branch b) (collect_names scrutinee) brs
-and collect_names_of_branch (b: branch)
-  : Tac (list name)
-  = let pat, body = b in
-    collect_names body @@ collect_names_of_pat pat
-and collect_names_of_pat (p: pattern)
-  : Tac (list name)
-  = match p with
-  | Pat_Cons fv l -> inspect_fv fv::(flatten (Tactics.map collect_names_of_pat (map fst l)))
-  | _ -> []
-
-let names_of_name (n: name): Tac (list name) 
-  = 
-  match lookup_typ (top_env ()) n with
-  | Some f -> (match inspect_sigelt f with
-           | Sg_Let _ _ _ _ d -> collect_names d
-           | _ -> [])
-  | None -> []
-
-let rec name_closure (names_todo: list name) (exclude: list name)
-  : Tac (list name)
-  = let excluded someName exclude = mem someName exclude in 
-    match names_todo with | [] -> []
-  | n::todo -> if excluded n exclude
-             then name_closure todo exclude
-             else let newTodo = names_of_name n in
-                  n :: name_closure (todo @@ newTodo) (n::exclude)
-
-
-
-
-
-
-let rec mfilter (f: 'a -> option 'b) (l: list 'a): list 'b
-  = match l with
-  | [] -> []
-  | hd::tl -> let r = mfilter f tl in match f hd with | Some v -> v::r | _ -> r
 
 let is_constructor (name: name)
   = Cons? name &&
@@ -334,47 +31,28 @@ let is_constructor (name: name)
             let firstLetter = String.sub last 0 1 in
             String.uppercase firstLetter = firstLetter))
 
-let inductive_name_from_constructor (n: name)
-  : Tac (list (name & typ))
-  = print ("--> " ^ implode_qn n ^ " : " ^ string_of_bool (is_constructor n));
-    if is_constructor n
+let inductive_name_from_constructor (n: name): Tac (list (name & typ))
+  = if is_constructor n
     then [n, tc (top_env ()) (pack (Tv_FVar (pack_fv n)))]
     else []
-    // let _, comp = collect_arr (tc (top_env ()) (pack (Tv_FVar (pack_fv n)))) in
-    // match inspect_comp comp with
-    // | C_Total ret _ -> 
-    //   let x,_   = collect_app
-    //   begin match lookup_typ (top_env ()) n with
-    //     | Some se -> begin match inspect_sigelt se with
-    //                     | Sg_Inductive n _ _ _ c -> [n]
-    //                     | _ -> print ("inductive_name_from_constructor("^implode_qn n^"): not a Sg_Inductive"); []
-    //                 end
-    //     | _ -> print ("inductive_name_from_constructor("^implode_qn n^"): cannot lookup the name"); []
-    //   end else []
-    // | _ -> print ("inductive_name_from_constructor("^implode_qn n^"): comp not total"); []
 
 let term_to_js_with_dep (t: term) (main_wrapper: js_expr -> js_stmt) (ignore_names: list name): Tac _
   = let names = name_closure (collect_names t) [] in
-    let namesxx = flatten (Tactics.map inductive_name_from_constructor names) in
+    let inductive_names = flatten (Tactics.map inductive_name_from_constructor names) in
     let sigelts': list (name & sigelt_view) = flatten (Tactics.map (fun n -> match lookup_typ (top_env ()) n with
       | Some se -> if mem n ignore_names then [] else [n, inspect_sigelt se]
       | None -> []
     ) names)
     in
-    // let sigeltsX = map (fun (n, se) -> 
-    //     match se with
-    //     | Sg_Let -> 
-    //     if is_constructor n
-    //     then 
-    //   ) sigelts' in
     let sigelts = map snd sigelts' in
-    let inductives = flatten (mfilter (function | Sg_Inductive _ _ _ _ c -> Some c | _ -> None) sigelts) in
-    // (match flatten (mfilter (fun (n, x) -> if Unk? x then Some n else None) sigelts) with
+    let inductives = flatten (mapOption (function | Sg_Inductive _ _ _ _ c -> Some c | _ -> None) sigelts) in
+    // (match flatten (mapOption (fun (n, x) -> if Unk? x then Some n else None) sigelts) with
     // | [] -> ()
     // | l -> fail (String.concat ", " ([] @@ l))
     // );
-    let dico: constructor_dico = mk_js_constructors (inductives @ namesxx) in
-    let lets = mfilter (fun (x: sigelt_view) -> if Sg_Let? x then Some #(s: _ {Sg_Let? s}) x else None) sigelts in
+    let dico = Tactics.map (fun (n, t) -> mk_js_constructor n t) (inductives @ inductive_names) in
+    let lets = mapOption (fun (x: sigelt_view) -> if Sg_Let? x then Some #(s: _ {Sg_Let? s}) x else None) sigelts in
     let lets_js = Tactics.map (fun x -> js_of_sg_view_let dico x) lets in
     let inductives_js = map js_of_constructor dico in
     sseq (inductives_js @ lets_js @ [main_wrapper (term_to_js_ast dico t)])
+
