Output.fst
@@ -2,6 +2,8 @@ module Output
 
 open FStar.String
 open FStar.List.Tot
+module R = FStar.Reflection.Builtins
+module RD = FStar.Reflection.Data
 
 let rec smaller' #t p ref (l: list t {l << ref /\ for_all p l})
   : (r: list (x: t {x << ref /\ p x}) { length l == length r })
@@ -15,19 +17,26 @@ let rec smaller #t ref (l: list t {l << ref})
   | [] -> []
   | hd::tl -> hd::smaller #t ref tl
 
-type mrange = int * int * int
+type position = | Position: col:nat -> line:nat -> position
+type range_info = | RangeInfo: file:string -> startp: position -> endp: position -> range_info
 
-type output =
-  | OPair: jump: bool -> left: string -> right: string -> content: list output -> output
-  | OQuote: string -> output
-  | OIdentitier: source: option mrange -> name: string -> output
-  | OKeyword: spaced: bool -> keyword: string -> output
-  | OSeparatedList: separator:output -> items: list output -> output
-  | ONest: list output -> output
+let range_to_range_info (r: range)
+  = let max (x y: int) = if x > y then x else y in
+    let h (t: int*int) = Position (max (fst t) 0) (max (snd t) 0) in
+    let r = R.inspect_range r in
+    RangeInfo r.RD.file_name (h r.RD.start_pos) (h r.RD.end_pos)
+
+type doc =
+  | OPair: jump: bool -> left: string -> right: string -> content: list doc -> doc
+  | OQuote: string -> doc
+  | OIdentitier: source: option range_info -> name: string -> doc
+  | OKeyword: spaced: bool -> keyword: string -> doc
+  | OSeparatedList: separator:doc -> items: list doc -> doc
+  | ONest: list doc -> doc
   | OEmpty
   
-let rec string_of_output' (tab: string) (o: output): Tot _ (decreases o)
-  = let map_self tab l = map (fun x -> string_of_output' tab x) l in 
+let rec string_of_doc' (tab: string) (o: doc): Tot _ (decreases o)
+  = let map_self tab l = map (fun x -> string_of_doc' tab x) l in 
     match o with
   | OPair jump left right content -> 
           let nl0 = if jump then "\n" ^ tab else "" in
@@ -38,10 +47,13 @@ let rec string_of_output' (tab: string) (o: output): Tot _ (decreases o)
   | OIdentitier _ name -> name
   | OKeyword spaced kwd -> let s = if spaced then " " else "" in
                           s ^ kwd ^ s
-  | OSeparatedList sep items -> (String.concat (string_of_output' tab sep) (map_self tab (smaller o items)))
+  | OSeparatedList sep items -> (String.concat (string_of_doc' tab sep) (map_self tab (smaller o items)))
   | ONest l -> String.concat "" (map_self tab (smaller o l))
   | OEmpty -> ""
 
-let string_of_output = string_of_output' ""
+let string_of_doc = string_of_doc' ""
 
+
+let (<+>) (a b: doc) =
+  
 
