JS.Ast.DSL.fst
@@ -1,0 +1,6 @@
+module JS.Ast.DSL
+
+open JS.Ast
+
+let (𝝺) = EAbs
+
