JS.Translate.Constructor.fst
@@ -1,0 +1,91 @@
+module JS.Translate.Constructor
+
+open FStar.List.Tot
+open JS.Ast
+open JS.Ast.Utils
+open JS.Translate.Helpers
+module O = Output
+
+type constructor
+  = { name: js_id
+    ; args: list (bool & js_id)
+    }
+type constructor_dico = list constructor
+    
+let mkCons (c: constructor) (args: list js_expr): js_expr
+  = ENew (EVar c.name) args
+
+let instanceOfCons (v: js_expr) (c: constructor): js_expr
+  = EBinaryOp JsBin_InstanceOf v (EGet (EVar c.name) (str "t"))
+
+let js_of_constructor (c: constructor)
+  = let thisCons = sFunction (Some c.name) (map snd c.args) (
+        let assign_arg (arg: js_id) = ( (EConst CThis `EGet` idname arg) `SAssign` EVar arg) in
+         sseq (map assign_arg (map snd c.args))
+      ) in
+    let mk_e body (explicit, arg) = 
+      if explicit then eFunction None [arg] (SReturn body)
+      else snd (make_implicit_abs arg body 0)
+    in
+    let mk_curried args body = fold_left mk_e body (rev args) in
+    let creatorLet = JSId None "creator" in
+    let creator = mk_curried c.args (
+      ENew (EVar c.name) (map EVar (map snd c.args))
+    ) in
+    SLet c.name (wrap_as_expr (
+       sseq
+         [ thisCons
+         ; SLet creatorLet creator
+         ; SAssign (EGet (EVar creatorLet) (str "t")) (EVar c.name)
+         ; SReturn (EVar creatorLet)
+         ]
+    ))
+
+type pattern_match =
+    | JPat_Constant : js_expr -> pattern_match
+    | JPat_Cons     : constructor -> list pattern_match -> pattern_match
+    | JPat_Var      : js_id -> pattern_match
+
+
+let rec js_condition_of_pattern_match (p: pattern_match) (head: js_expr): Tot js_expr (decreases p)
+  = match p with
+  | JPat_Constant e -> head ===. e
+  | JPat_Cons cons args -> fold_left (fun acc (pat, name) -> acc &&. js_condition_of_pattern_match (admit (); pat) (EGet head (idname name)))
+                                    (head `instanceOfCons` cons)
+                                    (zip args (map snd cons.args))
+  | JPat_Var _ -> EConst (CBool true)
+
+let rec js_bindings_of_pattern_match (p: pattern_match) (head: js_expr)
+  : Tot (list (js_id * js_expr)) (decreases p)
+  = match p with
+  | JPat_Constant e -> []
+  | JPat_Cons cons args -> fold_left (fun acc (pat, name) -> acc @ js_bindings_of_pattern_match (admit (); pat) (EGet head (idname name)))
+                                    []
+                                    (zip args (map snd cons.args))
+  | JPat_Var v -> [(v, head)]
+
+let js_of_pattern_match (p: pattern_match) (head: js_expr) (body: js_expr)
+  = let cond = js_condition_of_pattern_match p head in
+    let bindings = js_bindings_of_pattern_match p head in
+    let letClauses = fold_left (fun p (v, e) -> if SNoOp? p then SLet v e else p `SSeq` SLet v e) SNoOp bindings in
+    let body = letClauses `SSeq` SReturn body in
+    SIf cond body None
+
+
+let js_of_patterns_match (pb: list (pattern_match * js_expr)) (head: js_expr) (counter: nat)
+  : nat * js_expr
+  = let counter = counter + 1 in
+    counter,
+    wrap_as_expr begin
+      let let_temp = SLet (ReservedId counter) head in
+      let head = EVar (ReservedId counter) in
+      let branches = map (fun (pat, body) -> js_of_pattern_match pat head body) pb in
+      let_temp      `SSeq`
+      sseq branches `SSeq`
+      SThrow (
+        EBinaryOp JsBin_Plus
+          (str "Failed to pattern match ")
+          (head `EGet` str "constructor" `EGet` str "name")
+      )
+    end
+
