JS.Translate.Helpers.fst
@@ -1,0 +1,112 @@
+module JS.Translate.Helpers
+
+open FStar.Tactics
+open FStar.List.Tot
+open JS.Ast
+open JS.Ast.Utils
+module O = Output
+
+
+(*** Optionnal implicit support ***)
+/// If `enable_optional_implicit` is set to false, implicit and
+/// explicit binders in abstractions are treated the same. This should
+/// be the case: F* typechecker should always "fill the holes" of
+/// implicits, i.e. no implicit should be left
+/// uninstantiated. However, if you skip F* typecheck phase, you end
+/// up with term such as: `(fun #x y -> something) 3`, that is, with
+/// applications that "misses" implicits. The
+/// `enable_optional_implicit` flag makes the JS backend use a trick
+/// to skip the implicit that were left uninstantiated.
+let enable_optional_implicit = false
+let make_implicit_abs v (body: js_expr) (count: nat): nat & js_expr =
+  if enable_optional_implicit
+  then begin
+  let count = count + 1 in
+  // let  = ReservedId count in
+  // let count = count + 1 in
+  let bodyHolder = ReservedId count in
+  count,
+  EApp (eFunction None [] (
+    sseq
+      [ SLet v null
+      ; SLet bodyHolder body
+      ; SAssign (EGet (EVar bodyHolder) (str "feedImplicit")) (eFunction None [v] (
+                // TODO: here body is duplicated, we could circumvent
+                // this by having a binding `bodyHolder = v => body v`
+                // However, we should NOT set a new value to `v`
+                SReturn body
+        ))
+      ; SReturn (EVar bodyHolder)
+      ]
+  )) null []
+  end else count, (eFunction None [v] (SReturn body))
+
+let make_implicit_app f implicit_arg: js_expr
+  = if enable_optional_implicit
+    then
+    let feedImplicit = EGet f (str "feedImplicit") in
+    EApp (EBinaryOp JsBin_Or feedImplicit f) null [implicit_arg]
+    else EApp f null [implicit_arg]
+
+(*** Miscelanous helpers ***)
+
+let rec zip (a: list 'a) (b: list 'b) =
+  match a, b with
+  | a_hd::a_tl, b_hd::b_tl -> (a_hd,b_hd)::zip a_tl b_tl
+  | _ -> []
+
+let rec (@@) (#a: eqtype) (l1 l2: list a): Tot (list a) (decreases l2) = 
+  match l2 with | [] -> l1
+                | hd::tl -> if mem hd l1 then l1 @@ tl
+                          else (hd::l1) @@ tl
+
+let rec mapOption (f: 'a -> option 'b) (l: list 'a): list 'b
+  = match l with
+  | [] -> []
+  | hd::tl -> let r = mapOption f tl in match f hd with | Some v -> v::r | _ -> r
+
+let range_of_binder b: Tac range = range_of_term (binder_to_term b)
+
+(*** Names collection ***)
+/// The following just browse terms and collect any free
+/// variable. Note that types are irrelevant and thus discarded.
+let rec collect_names (t: term)
+  : Tac (list name)
+  = match inspect t with
+  | Tv_FVar  v -> [inspect_fv v]
+  | Tv_App   hd (arg, _) -> collect_names hd @@ collect_names arg
+  | Tv_Abs   _ body -> collect_names body
+  | Tv_Let _ _ _ def body -> collect_names def @@ collect_names body
+  | Tv_Arrow _ _ | Tv_Type _ | Tv_Refine _ _ | Tv_AscribedT _ _ _ | Tv_AscribedC _ _ _ | Tv_Uvar _ _ | Tv_Var _ | Tv_BVar _ | Tv_Const _ | Tv_Unknown -> []
+  | Tv_Match scrutinee brs -> Tactics.fold_left (fun l b -> l @@ collect_names_of_branch b) (collect_names scrutinee) brs
+and collect_names_of_branch (b: branch)
+  : Tac (list name)
+  = let pat, body = b in
+    collect_names body @@ collect_names_of_pat pat
+and collect_names_of_pat (p: pattern)
+  : Tac (list name)
+  = match p with
+  | Pat_Cons fv l -> inspect_fv fv::(flatten (Tactics.map collect_names_of_pat (map fst l)))
+  | _ -> []
+
+/// Given a toplevel name, `names_of_name` inspect the toplevel and
+/// returns a list of the names it directly use.
+let names_of_name (n: name): Tac (list name) 
+  = 
+  match lookup_typ (top_env ()) n with
+  | Some f -> (match inspect_sigelt f with
+           | Sg_Let _ _ _ _ d -> collect_names d
+           | _ -> [])
+  | None -> []
+
+/// `name_closure` computes a list of every names present directly or
+/// indirectly in the given toplevels.
+let rec name_closure (names_todo: list name) (exclude: list name)
+  : Tac (list name)
+  = let excluded someName exclude = mem someName exclude in 
+    match names_todo with | [] -> []
+  | n::todo -> if excluded n exclude
+             then name_closure todo exclude
+             else let newTodo = names_of_name n in
+                  n :: name_closure (todo @@ newTodo) (n::exclude)
+
