JS.Translate.Term.fst
@@ -1,0 +1,80 @@
+module JS.Translate.Term
+
+open FStar.Tactics
+open FStar.List.Tot
+open JS.Ast
+open JS.Ast.Utils
+open JS.Translate.Helpers
+open JS.Translate.Constructor
+module O = Output
+
+let c_unit =
+  { name = JSId None "Unit"
+  ; args = []
+  }
+
+let vconst_to_js_ast (c: vconst) =
+  match c with
+  | C_Unit      -> mkCons c_unit []
+  | C_Int     i -> EConst (CInt i)
+  | C_True      -> EConst (CBool true)
+  | C_False     -> EConst (CBool false)
+  | C_String  s -> EConst (CString s)
+  | C_Range   r -> EConst (CString "!RANGE!")
+  | C_Reify     -> EConst (CString "!REIFY!")
+  | C_Reflect _ -> EConst (CString "!REFLECT!")
+
+let rec branch_to_js_pattern_match (dico: constructor_dico) (pat: pattern): Tac _
+  = match pat with
+  | Pat_Constant vc -> JPat_Constant (vconst_to_js_ast vc)
+  | Pat_Cons fv args -> 
+         let name = fv_to_js_id fv in
+         ( match find (fun c -> js_id_eq c.name name) dico with
+         | Some c -> 
+             JPat_Cons c
+                       (Tactics.map (fun (a, _) -> branch_to_js_pattern_match dico a)
+                       (admit (); args))
+         | _ -> fail ("The constructor " ^ name_of_jsid name ^ " was not found in the supplied constructor dictionnary!" )
+         )
+  | Pat_Var bv | Pat_Wild bv | Pat_Dot_Term bv _ -> JPat_Var (bv_to_js_id bv)
+
+let rec term_to_js_ast' (dico: constructor_dico) (t: term) (count: nat)
+  : Tac (nat & js_expr)
+  = let recurse t count = term_to_js_ast' dico t count in
+    match inspect t with
+  | Tv_Var   v | Tv_BVar  v -> count, EVar (bv_to_js_id v)
+  | Tv_FVar  v -> count, EVar (fv_to_js_id v)
+  | Tv_App   hd (arg, aqual) -> 
+    let count, hd = recurse hd count in
+    let count, arg = recurse arg count in
+    count, 
+    ( match aqual with
+    | Q_Explicit -> EApp hd null [arg]
+    | _ -> make_implicit_app hd arg)
+  | Tv_Abs   bv body -> 
+    let count, body = recurse body count in
+    let jid = binder_to_js_id bv in
+    ( match inspect_binder bv with
+    | _, Q_Explicit -> count, EAbs [jid] body
+    | _ -> make_implicit_abs jid body count
+    )
+  | Tv_Arrow _ _ | Tv_Type _ | Tv_Refine _ _ | Tv_AscribedT _ _ _ | Tv_AscribedC _ _ _ | Tv_Uvar  _ _ -> count, null
+  | Tv_Const c -> count, vconst_to_js_ast c
+  | Tv_Let r _ bv def body -> 
+    let count, body = recurse body count in
+    let count, def = recurse def count in
+    (if r then elet' else elet_nonrec) (bv_to_js_id bv) def body count
+  | Tv_Unknown -> count, wrap_as_expr (SThrow (str "cannot translate Tv_Unknown"))
+  | Tv_Match scrutinee brs -> 
+             let count, branches = Tactics.fold_left (fun (count, l) (pat, body) -> 
+                 let count, t = recurse body count in
+                 count, l@[branch_to_js_pattern_match dico pat, t]
+               ) (0,[]) brs in
+             let count, scrutinee = recurse scrutinee count in
+             js_of_patterns_match branches scrutinee count
+
+let term_to_js_ast (dico: constructor_dico) (t: term)
+  : Tac js_expr
+  = snd (term_to_js_ast' dico t 0)
+
+
